Algoritmos Aproximados/Envasado.dfy/Algoritmo2AproximadoAux.dfy
@@ -1,0 +1,42 @@
+include "../../Especificaciones/Envasado/Envasado.dfy"
+include "EnvasadoKAproximado.dfy"
+
+//All bins are more than half full
+//Used locally
+predicate allMoreThanHalfFull(E: nat, I: multiset<multiset<nat>>)
+{
+    (forall M: multiset<nat> | M in I :: SumNat(M) * 2 > E)
+}
+
+//Only one bin in I is less than half full
+//Used locally
+predicate oneLessThanHalfFull(E: nat, I: multiset<multiset<nat>>)
+{
+    (exists M: multiset<nat> :: M in I && SumNat(M) * 2 <= E && (forall M': multiset<nat> | M' in I && SumNat(M') * 2 <= E :: M' == M)) 
+}
+
+lemma allMoreThanHalfFullImplies2Aproximated(A: multiset<nat>, E: nat, I: multiset<multiset<nat>>)
+requires isEnvasado(A, E, I)
+requires allMoreThanHalfFull(E, I) 
+ensures isKAproximatedBinPacking(A, E, I, 2)
+{
+    
+    assume false;
+}
+
+lemma oneLessThanHalfFullImplies2Aproximated(A: multiset<nat>, E: nat, I: multiset<multiset<nat>>)
+requires isEnvasado(A, E, I)
+requires oneLessThanHalfFull(E, I) 
+ensures isKAproximatedBinPacking(A, E, I, 2)
+{
+    assume false;
+}
+
+lemma atMostOneLessThanHalfImplies2Aproximated(A: multiset<nat>, E: nat, I: multiset<multiset<nat>>)
+requires isEnvasado(A, E, I)
+requires allMoreThanHalfFull(E, I) || oneLessThanHalfFull(E, I) 
+ensures isKAproximatedBinPacking(A, E, I, 2)
+{
+    if allMoreThanHalfFull(E, I){allMoreThanHalfFullImplies2Aproximated(A, E, I);}
+    else{oneLessThanHalfFullImplies2Aproximated(A, E, I); }
+}
