Algoritmos Aproximados/Envasado.dfy/Envasado2Aproximado.dfy
@@ -1,60 +1,11 @@
 include "../../Especificaciones/Envasado/Envasado.dfy"
 include "EnvasadoKAproximado.dfy"
 
-/*
+//We use the first fit strategy and check the elements in any order
+//At most only one bin is less than half full, thus we use most twice as many as in the optimal solution
 method binPacking2Aproximated(A: multiset<nat>, E: nat) returns (I: multiset<multiset<nat>>)
 //ensures isKAproximatedBinPacking(A, E, I, 2)
 {
-    //We use the first fit strategy and check the elements in any order
-    //At most only one bin is less than half full, thus we use most twice as many as in the optimal solution
-
-    //Variable initialization
-    //bins will hold the solution, expressed as a multiset of tupples that each represent a bin, in which the first element is the its contents and the second is its capacity
-    var bins: multiset<(multiset<nat>, nat)> := multiset{};
-    //iterateMultiset exists to let us iterate over all the elements in A, one by one
-    var iterateMultiset: multiset<nat> := A;
-    I := multiset{};
-
-    while iterateMultiset != multiset{}
-    decreases iterateMultiset
-    //at most  one bin is less than half full
-    {
-        var currElement: nat := pickMultiset(iterateMultiset);
-        var binsIterate := bins;
-        var fit: bool := false; 
-        while !fit && binsIterate != multiset{}
-        {
-            var currBin: (multiset<nat>, nat)  := pickMultiset(binsIterate);
-            if currBin.1 + currElement < E {
-                //mejor forma?
-                bins := bins - multiset{currBin};
-                var newBin := (currBin.0 + multiset{currElement}, currBin.1 + currElement);
-                bins := bins + multiset{newBin};
-                fit := true;
-            }
-            binsIterate := binsIterate - multiset{currBin};
-        }
-        if !fit {
-            var copyBins := bins;
-            bins := bins + multiset{(multiset{currElement}, currElement)};
-        }
-        iterateMultiset := iterateMultiset - multiset{currElement};
-    }
-    while bins != multiset{}
-    {
-        var currBin := pickMultiset(bins);
-        I := I + multiset{currBin.0};
-        bins := bins - multiset{currBin};
-    }
-}
-*/
-
-method binPacking2AproximatedSeq(A: multiset<nat>, E: nat) returns (I: multiset<multiset<nat>>)
-//ensures isKAproximatedBinPacking(A, E, I, 2)
-{
-    //We use the first fit strategy and check the elements in any order
-    //At most only one bin is less than half full, thus we use most twice as many as in the optimal solution
-
     //Variable initialization
     //bins will hold the solution, expressed as a multiset of tupples that each represent a bin, in which the first element is the its contents and the second is its capacity
     var bins: seq<multiset<nat>> := [];
@@ -74,17 +25,17 @@ method binPacking2AproximatedSeq(A: multiset<nat>, E: nat) returns (I: multiset<
         invariant |bins| == |capacity|
         {
             if capacity[i] + currElement < E {
-                //mejor forma?
                 bins := bins[i := (bins[i] + multiset{currElement})];
                 fit := true;
             }
             i := i + 1;
         }
+        //If no fit was found we must create another bin
         if !fit {
             bins := bins + [multiset{currElement}];
             capacity := capacity + [currElement];
         }
         iterateMultiset := iterateMultiset - multiset{currElement};
     }
-    I := multiset(bins[..]);
+    I := multiset(bins);
 }
