Algoritmos Aproximados/Envasado.dfy/EnvasadoKAproximado.dfy
@@ -1,5 +1,6 @@
 include "../../Especificaciones/Envasado/Envasado.dfy"
 
+//Definition of what it means for a solution to be K-Aproximated in the Bin Packing Problem
 ghost predicate isKAproximatedBinPacking(A : multiset<nat>, E : nat, I:multiset<multiset<nat>>, k: nat)
 {
        isEnvasado(A, E, I)
