Especificaciones/Auxiliar/Graph.dfy
@@ -1,21 +1,16 @@
 include "SetFacts.dfy"
 
-
+//Definition of Graph, Edge, and Node types
 type Node = nat
 type Edge = set<Node>
-
 type Graph = (set<Node>, set<Edge>)
 
-function complement (graph:Graph) : (r:Graph)
-requires isValidGraph(graph)
-ensures isValidGraph(r) 
-{
-    var allEdges:set<Edge> := (set n1,n2 | n1 in graph.0 && n2 in graph.0 && n1 != n2 :: {n1,n2});
-    var complementGraph:Graph := (graph.0, allEdges-graph.1);
-    (complementGraph)
-}
+/////////////////////////////////////////////////
+//                  Functions                  //
+/////////////////////////////////////////////////
 
-
+//Returns true iff the value of graph represents a valid graph
+//Used whenever we have to work with graphs
 predicate isValidGraph(graph: Graph)
 {
     forall e | e in graph.1 :: 
@@ -25,6 +20,9 @@ predicate isValidGraph(graph: Graph)
 }
 
 //Returns true iff A is a subgraph of B
+//Used in CliqueProperties
+//        POCToPC
+//        POCToPCAux
 predicate isSubGraph(A: Graph, B: Graph)
 requires isValidGraph(A)
 requires isValidGraph(B)
@@ -32,48 +30,123 @@ requires isValidGraph(B)
     A.0 <= B.0 && A.1 <= B.1
 }
 
-lemma corollaryToValidity(graph: Graph, S: set<Node>)
+//Returns the set of edges incident on vertex node
+//Used locally
+//     in OptimalCoverPropertiesSplit 
+//     in POCToPCV
+//     in POCToPCVRemoveVertex
+//     in RemoveVertexAux 
+function incidentEdges(graph: Graph, node: Node) : (S: set<Edge>)
 requires isValidGraph(graph)
-requires graph.0 * S == {}
-ensures forall n: Node, e: Edge | n in S && e in graph.1 :: n !in e
-{ }
-
-lemma existenceImpliesNonEmpty<T>(A: set<T>, B: set<set<T>>)
-requires forall x: T | x in A :: (exists y: set<T> :: y in B && x in y)
-ensures forall x: T | x in A :: (set y: set<T> | y in B && x in y :: y) != {}
-{ 
-    if exists x: T :: x in A && (set y: set<T> | y in B && x in y :: y) == {} {
-        var x: T :| x in A && (set y: set<T> | y in B && x in y :: y) == {}; 
-        var setX: set<set<T>> := (set y: set<T> | y in B && x in y :: y);
-        assert forall y: set<T> | y in B && x in y :: y in setX;
-        assert setX == {};
-        assert forall y: set<T> | y in B :: x !in y;
-    }
-}
-
-lemma intersect(s: set<Node>, graph:Graph, e: Edge, u: Node, v: Node)
-requires isValidGraph(graph)
-requires e in graph.1
-requires u in graph.0 && v in graph.0 && u != v && e == {u,v}
-requires s <= graph.0
-ensures |s * e| <= 2 
-ensures s * e == {} || s * e == {u} || s * e == {v} || s * e == e 
+ensures forall e: Edge | e in S :: |e| == 2
+ensures forall e: Edge | e in S :: exists n: Node :: n in graph.0 && n in e && n != node
+ensures forall e: Edge | e in graph.1 :: e in S <==> node in e
+ensures forall e: Edge | e in graph.1 && node in e :: e in S
 {
- 
-    if (u !in s && v !in s) {
-        assert s * e == {}; 
-     }
-     else if (u in s && v !in s) {
-        assert s * e == {u};
-     }
-     else if (u !in s && v in s) {
-        assert s * e == {v};
-     }
-     else if (u in s && v in s) {
-        assert s * e == {u,v};}
-
+    (set edge: Edge | edge in graph.1 && node in edge :: edge)
 }
 
+//Returns the set of nodes adjacent to v
+//Used locally 
+//     in SplitVertexAux 
+function neighborsOf(graph: Graph, v: Node) : (S: set<Node>)
+requires isValidGraph(graph)
+ensures forall n: Node | n in S :: n in graph.0 && n != v
+{
+    (set node: Node | node in graph.0  && {v, node} in graph.1 :: node)
+}
+
+//Returns a graph without the vertex v and the edges incident on it
+//Used locally
+//     in POCToPC
+//     in POCToPCAux
+//     in POCVToPCVRemoveVertex
+function removeVertex(graph: Graph, v: Node): (graph': Graph) 
+requires isValidGraph(graph)
+ensures isValidGraph(graph')
+ensures forall e: Edge | e in graph.1 :: v in e <==> e !in graph'.1
+ensures forall e: Edge | e in graph.1 :: v !in e <==> e in graph'.1
+{
+    (graph.0 - {v}, graph.1 - incidentEdges(graph, v))
+}
+
+
+//Given a graph and a vertex, splits the vertex to create various vertices that maintain the incident edges
+//Used in POCVToPCVSplitVertex
+//     in SplitVertexAux
+function splitVertex(graph: Graph, v: Node): (r: Graph)
+requires isValidGraph(graph) 
+ensures isValidGraph(r)
+ensures forall n: Node | n in (r.0 - graph.0) :: |(set e: Edge | e in (r.1) && n in e :: e)| == 1
+{
+    
+    //If it belongs to the graph
+    if v in graph.0 then 
+        //The vertex is "split" such that all those edges still exist but connect to different new nodes
+        var edgesToChange: set<Edge> := incidentEdges(graph, v);
+        var newNodes: set<Node> := addMultipleGreater(graph.0, |edgesToChange|); 
+        assert newNodes * graph.0 == {};
+        assert(|newNodes| == |edgesToChange|);
+        incidentEdgesContainsNeighbors(graph, v, edgesToChange);
+        //newSplitEdges(graph, newNodes, edgesToChange, v);
+        var setNewEdges: set<Edge> := (set node1: Node, node2: Node | node1 in newNodes && node2 in neighborsOf(graph, v) && numberOfLesser(newNodes, node1) == numberOfLesser(neighborsOf(graph, v), node2) :: {node1, node2});
+        var g := ((graph.0 - {v} + newNodes), (graph.1 - edgesToChange + setNewEdges));
+
+        //Proof for isValidGraph(r)
+        assert isValidGraph(g) by {
+            assert forall e | e in setNewEdges :: |e| == 2;
+            assert forall e | e in setNewEdges :: (exists a, b :: a in newNodes && b in (graph.0 - {v}) && a != b && e == {a, b});
+            assert newNodes <= g.0;
+            assert isValidGraph((graph.0 - {v}, graph.1 - incidentEdges(graph, v)));
+            assert g.1 == graph.1 - incidentEdges(graph, v) + setNewEdges;
+            assert forall e: Edge | e in graph.1 :: (|e| == 2 && exists u,v :: u in graph.0 && v in graph.0 && u != v && e == {u,v});
+        }
+        
+        //Proof for forall n: Node | n in (r.0 - graph.0) :: |(set e: Edge | e in (r.1) && n in e :: e)| == 1
+        forall n: Node | n in (g.0 - graph.0) 
+        ensures |(set e: Edge | e in g.1 && n in e :: e)| == 1
+        {    
+            //assert newNodes * graph.0 == {};
+            ghost var incidents: set<Edge> := incidentEdges(graph, v);
+            //assert (g.0 - graph.0) == newNodes;
+            //assert newNodes * graph.0 == {}; 
+            assert forall node: Node, e: Edge | e in graph.1 && node in e :: node in graph.0; 
+            //assert forall e: Edge | e in graph.1 :: n !in e;
+            //assert (set e: Edge | e in (graph.1 - incidents) && n in e :: e) <= graph.1;
+            //assert (set e: Edge | e in (graph.1 - incidents) && n in e :: e) == {};
+            //assert |(set e: Edge | e in (graph.1 - incidents) && n in e :: e)| == 0;
+            asManyNewNodesAsEdges(graph, v, newNodes, setNewEdges); 
+            //assert |(set e: Edge | e in setNewEdges && n in e :: e)| == 1;
+            //assert g.1 == graph.1 - incidentEdges(graph, v) + setNewEdges;
+            ghost var setG := (set e: Edge | e in ((graph.1 - incidents) + setNewEdges) && n in e :: e);
+            ghost var nInNewEdges: set<Edge> := (set e: Edge | e in setNewEdges && n in e :: e);
+            ghost var nInOldEdges: set<Edge> := (set e: Edge | e in (graph.1 - incidents) && n in e :: e);
+            calc =={
+                setG; 
+                (set e: Edge | (e in ((graph.1 - incidents) + setNewEdges)) && n in e :: e);
+                { setComprehensionUnion((graph.1 - incidents),setNewEdges,n);} 
+                (set e: Edge | e in (graph.1 - incidents) && n in e :: e) + 
+                (set e: Edge | e in setNewEdges && n in e :: e);                
+                nInOldEdges + nInNewEdges;
+            }
+            assert setG == nInOldEdges + nInNewEdges;
+            cardinalityUnion(nInOldEdges, nInNewEdges, setG);
+        }
+        
+        g
+        
+    //If the vertex does not belong to the graph, it remains unchanged
+    else graph
+}
+
+//////////////////////////////////////////////////
+//                    Lemmas                    //
+//////////////////////////////////////////////////
+
+//The result of removing a vertex and its incident edges from a graph is another valid graph
+//Used in POCToPC
+//        POCVToPCVSplitVertex
+//        POCVToPCVRemoveVertex
 lemma validSubgraph(graph : Graph, v : Node, graph': Graph)
 requires isValidGraph(graph)
 requires graph'.0 == graph.0 - { v }
@@ -81,148 +154,8 @@ requires graph'.1 == graph.1 - incidentEdges(graph,v)
 ensures isValidGraph(graph')
 {}
 
-function pickEdgeFromNode(newNodes: set<Node>, edgesToChange: set<Edge>, removedNode: Node): (e: Edge)
-requires |newNodes| > 0 && |edgesToChange| == |newNodes|
-requires forall edge: Edge | edge in edgesToChange :: removedNode in edge && |edge| == 2
-ensures e in edgesToChange
-{
-    assert |edgesToChange| > 0;
-    var allIncidentNodes: set<Node> := flatten(edgesToChange) - {removedNode};
-    assert forall E: Edge | E in edgesToChange :: |(E - {removedNode})| > 0;
-    assert forall E: Edge | E in edgesToChange :: (exists n: Node :: n != removedNode && n in E);
-    assert exists S: Edge :: S in edgesToChange && |S| == 2 && (exists n: Node :: n != removedNode && n in S) && S <= flatten(edgesToChange) ;
-    assert |allIncidentNodes| > 0;
-    var maxNode: Node := pickMax(allIncidentNodes);
-    assert maxNode in allIncidentNodes;
-    var pickedEdge: Edge := {removedNode, maxNode};
-    assert exists edge: Edge :: edge in edgesToChange && maxNode in edge && removedNode in edge && |edge| == 2;
-    assert exists edge: Edge :: edge in edgesToChange && edge >= {removedNode, maxNode};
-    cardinalityLemma2();
-    assert exists edge: Edge :: edge in edgesToChange && edge == pickedEdge;
-    assert pickedEdge in edgesToChange;
-    pickedEdge
-}
-/*
-function {:only} newSplitEdgesRec(graph: Graph, newNodes: set<Node>, newNodesRemaining: set<Node>, edgesToChange: set<Edge>, removedNode: Node, setAnalyzedNodes: set<Node>, setCreatedEdges: set<Edge>): (r: set<Edge>)
-requires isValidGraph(graph)
-requires removedNode in graph.0
-requires edgesToChange <= graph.1
-requires forall edge: Edge | edge in edgesToChange :: removedNode in edge && |edge| == 2
-requires removedNode !in newNodes
-requires |edgesToChange| == |newNodesRemaining|
-requires |setAnalyzedNodes| == |setCreatedEdges|
-requires newNodes * graph.0 == {}
-requires newNodesRemaining <= newNodes
-requires newNodesRemaining * graph.0 == {}
-requires setAnalyzedNodes * newNodesRemaining == {}
-requires setAnalyzedNodes + newNodesRemaining == newNodes
-requires forall e: Edge | e in edgesToChange :: (exists n: Node :: n in e && n in neighborsOf(graph, removedNode))
-requires forall n: Node | n in setAnalyzedNodes :: ((exists e: Edge :: e in setCreatedEdges && n in e))  
-requires forall n: Node, e: Edge | n !in setAnalyzedNodes && n !in (graph.0 - {removedNode}) && e in setCreatedEdges :: n !in e
-requires forall n: Node | n in setAnalyzedNodes :: ((exists e: Edge :: e in setCreatedEdges && n in e)) 
-decreases edgesToChange
-ensures forall e: Edge | e in r :: |e| == 2 
-ensures forall n: Node, e: Edge | n !in newNodesRemaining && n !in (graph.0 - {removedNode}) && e in r :: n !in e 
-ensures forall e: Edge | e in r :: (exists node1: Node, node2: Node :: node1 in newNodes && node2 in (graph.0 - {removedNode}) && e == {node1, node2}) 
-ensures forall n: Node | n in newNodes :: ((exists e: Edge :: e in (r + setCreatedEdges) && n in e))
-//ensures forall e: Edge | e in r :: (exists n: Node :: n in e && n in neighborsOf(graph, removedNode))
-ensures forall n: Node | n in newNodesRemaining :: (|(set e: Edge | e in r && n in e :: e)| == 1)
-{
-    if edgesToChange == {} then 
-        assert setAnalyzedNodes == newNodes;
-        assert forall n: Node | n in setAnalyzedNodes :: (exists e: Edge :: e in setCreatedEdges && n in e);
-        {}
-    else
-        //Functionality
-        var node: Node := pickMax(newNodesRemaining);
-        var changedEdge: Edge := pickEdgeFromNode(newNodesRemaining, edgesToChange, removedNode);
-        var edge' := changedEdge - {removedNode};
-        var edge'' := edge' + {node};
-        assert node !in setAnalyzedNodes;
-        assert edge'' !in setCreatedEdges;
-        var remainingEdges: set<Edge> := newSplitEdgesRec(graph, newNodes, newNodesRemaining - {node}, edgesToChange - {changedEdge}, removedNode, setAnalyzedNodes + {node}, setCreatedEdges + {edge''});
-        var rv: set<Edge> := {edge''} + remainingEdges;
-
-        //No particular proof needed
-        /*assert forall e: Edge | e in rv :: |e| == 2 ;
-        assert forall n: Node, e: Edge | n !in newNodesRemaining && n !in (graph.0 - {removedNode}) && e in rv :: n !in e; 
-        assert forall n: Node | n in newNodes :: ((exists e: Edge :: e in (rv + setCreatedEdges) && n in e));
-        */
-
-        //Proof for forall e: Edge | e in r :: (exists node1: Node, node2: Node :: node1 in newNodes && node2 in (graph.0 - {removedNode}) && e == {node1, node2})  
-        assert exists n: Node :: n in (graph.0 - {removedNode}) && n in edge';
-        ghost var nodeFromGraph: Node :| nodeFromGraph in (graph.0 - {removedNode}) && nodeFromGraph in edge';
-        assert edge'' == {node, nodeFromGraph};
-        assert forall e: Edge | e in rv :: (exists node1: Node, node2: Node :: node1 in newNodes && node2 in (graph.0 - {removedNode}) && e == {node1, node2});
-        assume false;
-
-        //Proof for forall n: Node | n in newNodes :: (|(set e: Edge | e in r && n in e :: e)| == 1)
-        
-        ghost var setEdge: set<Edge> := (set e: Edge | e in {edge''} && node in e :: e);
-        assert setEdge == {edge''};
-        ghost var setEdgeEmpty := (set e: Edge | e in remainingEdges && node in e :: e);
-        assert setEdgeEmpty == {};
-        assert (set e: Edge | e in rv && node in e :: e) == setEdge + setEdgeEmpty;
-        cardinalitySum(setEdge, setEdgeEmpty);
-        assert |setEdge + setEdgeEmpty| == 1;
-        assert rv == rv;
-        assert rv == (setEdge + remainingEdges);
-        assert forall e: Edge :: e in rv <==> e in rv;
-        equalityBelonging(rv, (setEdge + remainingEdges));
-        assert forall e: Edge :: e in rv <==> e in (setEdge + remainingEdges);
-        //DUDA
-        assert forall e: Edge :: e in (set e: Edge | e in rv && node in e :: e) <==> (e in (setEdge + remainingEdges) && node in e);
-        assume false;
-        assert (set e: Edge | e in rv && node in e :: e) == setEdge + setEdgeEmpty;
-        cardinalitySum(setEdge, setEdgeEmpty);
-        assert |setEdge + setEdgeEmpty| == 1;
-        equialityImpliesSameCardinal((set e: Edge | e in rv && node in e :: e), (setEdge + setEdgeEmpty));
-        assert |(set e: Edge | e in rv && node in e :: e)| == |setEdge + setEdgeEmpty|;
-        assert forall n: Node | n in newNodesRemaining && n == node :: (|(set e: Edge | e in rv && n in e :: e)| == 1);
-        assert forall n: Node, e: Edge | n in newNodesRemaining && n != node && e in setCreatedEdges :: n !in e;
-        assert forall n: Node | n in newNodes :: ((exists e: Edge :: e in (rv + setCreatedEdges) && n in e));
-        assert forall n: Node, e: Edge | n in newNodesRemaining && n != node && e in setCreatedEdges :: n !in e;
-        
-        /*
-        assert forall n: Node | n in newNodesRemaining :: (|(set e: Edge | e in rv && n in e :: e)| >= 1) by {
-            //assert forall n: Node | n in newNodes :: ((exists e: Edge :: e in (rv + setCreatedEdges) && n in e));
-            //assert forall n: Node | n in newNodesRemaining :: ((exists e: Edge :: e in (rv + setCreatedEdges) && n in e));
-            //assert forall n: Node | n in newNodesRemaining :: n !in setAnalyzedNodes && n !in graph.0 - {removedNode};
-            //assert forall n: Node, e: Edge | n !in setAnalyzedNodes && n !in (graph.0 - {removedNode}) && e in setCreatedEdges :: n !in e;
-            //assert forall n: Node, e: Edge | n in newNodesRemaining && e in setCreatedEdges :: n !in e;
-            //assert forall n: Node | n in newNodesRemaining :: (exists e: Edge :: e in rv && n in e);
-            //existenceImpliesNonEmpty(newNodesRemaining, rv);
-            //assert forall n: Node | n in newNodesRemaining :: (set e: Edge | e in rv && n in e :: e) != {};
-        }
-        */
-        rv
-        
-}
-*/
-
-/*
-function newSplitEdges(graph: Graph, newNodes: set<Node>, edgesToChange: set<Edge>, removedNode: Node): (r: set<Edge>)
-requires isValidGraph(graph)
-requires removedNode in graph.0
-requires edgesToChange <= graph.1
-requires forall edge: Edge | edge in edgesToChange :: removedNode in edge && |edge| == 2
-requires removedNode !in newNodes
-requires |edgesToChange| == |newNodes|
-requires newNodes * graph.0 == {}
-requires forall e: Edge | e in edgesToChange :: (exists n: Node :: n in e && n in neighborsOf(graph, removedNode))
-decreases edgesToChange
-ensures forall e: Edge | e in r :: |e| == 2 
-ensures forall n: Node, e: Edge | n !in newNodes && n !in (graph.0 - {removedNode}) && e in r :: n !in e 
-ensures forall e: Edge | e in r :: (exists node1: Node, node2: Node :: node1 in newNodes && node2 in (graph.0 - {removedNode}) && e == {node1, node2}) 
-//ensures forall n: Node | n in newNodes :: ((exists e: Edge :: e in r && n in e))
-ensures forall e: Edge | e in r :: (exists n: Node :: n in e && n in neighborsOf(graph, removedNode))
-ensures forall n: Node | n in newNodes :: (|(set e: Edge | e in r && n in e :: e)| == 1)
-{
-    var setAnalyzedNodes: set<Node> := {};    
-    newSplitEdgesRec(graph, newNodes, newNodes, edgesToChange, removedNode, {}, {})  
-}
-*/
-
+//All adjacent nodes to node n belong to some edge incident on n
+//Used locally 
 lemma incidentEdgesContainsNeighbors(g: Graph, n: Node, I: set<Edge>)
 requires isValidGraph(g)
 requires incidentEdges(g, n) == I
@@ -236,19 +169,10 @@ ensures forall e: Edge | e in I :: (exists node: Node :: node in e && node in ne
    }
 }
 
-function incidentEdges(graph: Graph, node: Node) : (S: set<Edge>)
-requires isValidGraph(graph)
-ensures forall e: Edge | e in S :: |e| == 2
-ensures forall e: Edge | e in S :: exists n: Node :: n in graph.0 && n in e && n != node
-ensures forall e: Edge | e in graph.1 :: e in S <==> node in e
-ensures forall e: Edge | e in graph.1 && node in e :: e in S
-{
-    (set edge: Edge | edge in graph.1 && node in edge :: edge)
-}
-
+//All adjacent nodes to n are connected to it by an edge
+//Used in SplitVertexAux
 lemma neighborsAreConnected(g: Graph, n: Node, S: set<Node>)
 requires isValidGraph(g)
-//requires n in g.0
 requires S == neighborsOf(g, n)
 ensures forall m: Node | n in S :: {m, n} in g.1 
 {
@@ -257,55 +181,8 @@ ensures forall m: Node | n in S :: {m, n} in g.1
     }
 }
 
-function neighborsOf(graph: Graph, v: Node) : (S: set<Node>)
-requires isValidGraph(graph)
-ensures forall n: Node | n in S :: n in graph.0 && n != v
-{
-    (set node: Node | node in graph.0  && {v, node} in graph.1 :: node)
-}
-
-function removeVertex(graph: Graph, v: Node): (graph': Graph) 
-requires isValidGraph(graph)
-//requires v in graph.0
-ensures isValidGraph(graph')
-ensures forall e: Edge | e in graph.1 :: v in e <==> e !in graph'.1
-ensures forall e: Edge | e in graph.1 :: v !in e <==> e in graph'.1
-{
-    (graph.0 - {v}, graph.1 - incidentEdges(graph, v))
-}
-
-function addedSplitNodes(graph: Graph, v: Node): (S: set<Node>)
-requires isValidGraph(graph) 
-{
-    if v in graph.0 && (exists e: Edge | e in graph.1 :: v in e ) then 
-        //The vertex is "split" such that all those edges still exist but connect to different new nodes
-        var edgesToChange: set<Edge> := incidentEdges(graph, v);
-        var newNodes: set<Node> := addMultipleGreater(graph.0, |edgesToChange|); 
-        newNodes
-    //If the vertex does not belong to the graph or the vertex is not present in any edge, there are no new nodes
-    else {}
-}
-
-lemma removeVertexValid(g: Graph, v: Node)
-requires isValidGraph(g)
-requires v in g.0
-ensures isValidGraph((g.0 - {v}, g.1 - incidentEdges(g, v)))
-{
-    assert forall e | e in g.1 :: (|e| == 2 && exists u,v :: u in g.0 && v in g.0 && u != v && e == {u,v}); 
-}
-
-lemma notAVertexImpliesNotInAnEdge(graph: Graph, n: Node)
-requires isValidGraph(graph)
-requires n !in graph.0
-ensures forall e: Edge | e in graph.1 :: n !in e
-{ }
-
-lemma notAVertexImpliesNotInAnEdgeSet(graph: Graph, S: set<Node>)
-requires isValidGraph(graph)
-requires forall n: Node | n in S :: n !in graph.0
-ensures forall e: Edge, n: Node | e in graph.1 && n in S :: n !in e
-{ }
-
+//There are as many incident edges as adjacent nodes 
+//Used locally
 lemma aNeighborForEachIncidentEdge(graph: Graph, node: Node)
 decreases graph.0
 requires isValidGraph(graph)
@@ -344,6 +221,8 @@ ensures |incidentEdges(graph, node)| == |neighborsOf(graph, node)|
     }
 }
 
+//All new nodes are contained by exactly one new edge, and thus, there are as many new nodes as edges
+//Used locally
 lemma asManyNewNodesAsEdges(graph: Graph, v: Node, newNodes: set<Node>, setNewEdges: set<Edge>)
 requires isValidGraph(graph)
 requires v in graph.0
@@ -422,69 +301,103 @@ ensures |newNodes| == |setNewEdges|
     }
 }
 
-//Given a graph and a vertex
-function splitVertex(graph: Graph, v: Node): (r: Graph)
-requires isValidGraph(graph) 
-ensures isValidGraph(r)
-ensures forall n: Node | n in (r.0 - graph.0) :: |(set e: Edge | e in (r.1) && n in e :: e)| == 1
-{
-    
-    //If it belongs to the graph
-    if v in graph.0 then 
-        //The vertex is "split" such that all those edges still exist but connect to different new nodes
-        var edgesToChange: set<Edge> := incidentEdges(graph, v);
-        var newNodes: set<Node> := addMultipleGreater(graph.0, |edgesToChange|); 
-        assert newNodes * graph.0 == {};
-        assert(|newNodes| == |edgesToChange|);
-        incidentEdgesContainsNeighbors(graph, v, edgesToChange);
-        //newSplitEdges(graph, newNodes, edgesToChange, v);
-        var setNewEdges: set<Edge> := (set node1: Node, node2: Node | node1 in newNodes && node2 in neighborsOf(graph, v) && numberOfLesser(newNodes, node1) == numberOfLesser(neighborsOf(graph, v), node2) :: {node1, node2});
-        var g := ((graph.0 - {v} + newNodes), (graph.1 - edgesToChange + setNewEdges));
+//////////////////////////////////////////////////
+//               Currently Unused               //
+//////////////////////////////////////////////////
+/*
 
-        //Proof for isValidGraph(r)
-        assert isValidGraph(g) by {
-            assert forall e | e in setNewEdges :: |e| == 2;
-            assert forall e | e in setNewEdges :: (exists a, b :: a in newNodes && b in (graph.0 - {v}) && a != b && e == {a, b});
-            assert newNodes <= g.0;
-            removeVertexValid(graph, v);
-            assert isValidGraph((graph.0 - {v}, graph.1 - incidentEdges(graph, v)));
-            assert g.1 == graph.1 - incidentEdges(graph, v) + setNewEdges;
-            assert forall e: Edge | e in graph.1 :: (|e| == 2 && exists u,v :: u in graph.0 && v in graph.0 && u != v && e == {u,v});
-        }
-        
-        //Proof for forall n: Node | n in (r.0 - graph.0) :: |(set e: Edge | e in (r.1) && n in e :: e)| == 1
-        forall n: Node | n in (g.0 - graph.0) 
-        ensures |(set e: Edge | e in g.1 && n in e :: e)| == 1
-        {    
-            //assert newNodes * graph.0 == {};
-            ghost var incidents: set<Edge> := incidentEdges(graph, v);
-            //assert (g.0 - graph.0) == newNodes;
-            //assert newNodes * graph.0 == {}; 
-            assert forall node: Node, e: Edge | e in graph.1 && node in e :: node in graph.0; 
-            //assert forall e: Edge | e in graph.1 :: n !in e;
-            //assert (set e: Edge | e in (graph.1 - incidents) && n in e :: e) <= graph.1;
-            //assert (set e: Edge | e in (graph.1 - incidents) && n in e :: e) == {};
-            //assert |(set e: Edge | e in (graph.1 - incidents) && n in e :: e)| == 0;
-            asManyNewNodesAsEdges(graph, v, newNodes, setNewEdges); 
-            //assert |(set e: Edge | e in setNewEdges && n in e :: e)| == 1;
-            //assert g.1 == graph.1 - incidentEdges(graph, v) + setNewEdges;
-            ghost var setG := (set e: Edge | e in ((graph.1 - incidents) + setNewEdges) && n in e :: e);
-            ghost var nInNewEdges: set<Edge> := (set e: Edge | e in setNewEdges && n in e :: e);
-            ghost var nInOldEdges: set<Edge> := (set e: Edge | e in (graph.1 - incidents) && n in e :: e);
-            calc =={
-                setG; 
-                (set e: Edge | (e in ((graph.1 - incidents) + setNewEdges)) && n in e :: e);
-                { setComprehensionUnion((graph.1 - incidents),setNewEdges,n);} 
-                (set e: Edge | e in (graph.1 - incidents) && n in e :: e) + 
-                (set e: Edge | e in setNewEdges && n in e :: e);                
-                nInOldEdges + nInNewEdges;
-            }
-            assert setG == nInOldEdges + nInNewEdges;
-            cardinalityUnion(nInOldEdges, nInNewEdges, setG);
-        }
-        
-        g
-        
-    //If the vertex does not belong to the graph, it remains unchanged
-    else graph
+//Returns he complementary Graph, vertices stay the same, but in r two nodes are connected iff they are not connected in graph
+function complement (graph:Graph) : (r:Graph)
+requires isValidGraph(graph)
+ensures isValidGraph(r) 
+{
+    var allEdges:set<Edge> := (set n1,n2 | n1 in graph.0 && n2 in graph.0 && n1 != n2 :: {n1,n2});
+    var complementGraph:Graph := (graph.0, allEdges-graph.1);
+    (complementGraph)
 }
+
+//The intersection of a subset of the graph's vertices with one of its edges contains none, either, or bot of the vertices in said edge
+lemma intersect(s: set<Node>, graph:Graph, e: Edge, u: Node, v: Node)
+requires isValidGraph(graph)
+requires e in graph.1
+requires u in graph.0 && v in graph.0 && u != v && e == {u,v}
+requires s <= graph.0
+ensures |s * e| <= 2 
+ensures s * e == {} || s * e == {u} || s * e == {v} || s * e == e 
+{
+ 
+    if (u !in s && v !in s) {
+        assert s * e == {}; 
+     }
+     else if (u in s && v !in s) {
+        assert s * e == {u};
+     }
+     else if (u !in s && v in s) {
+        assert s * e == {v};
+     }
+     else if (u in s && v in s) {
+        assert s * e == {u,v};}
+
+}
+
+//Given a set of edges all of which contain vertex removedNode, returns the edge that conatins the greatest vertex different from removedNode
+function pickEdgeFromNode(edgesToChange: set<Edge>, removedNode: Node): (e: Edge)
+requires |edgesToChange| > 0
+requires forall edge: Edge | edge in edgesToChange :: removedNode in edge && |edge| == 2
+ensures e in edgesToChange
+{
+    assert |edgesToChange| > 0;
+    var allIncidentNodes: set<Node> := Union(edgesToChange) - {removedNode};
+    assert forall E: Edge | E in edgesToChange :: |(E - {removedNode})| > 0;
+    assert forall E: Edge | E in edgesToChange :: (exists n: Node :: n != removedNode && n in E);
+    assert exists S: Edge :: S in edgesToChange && |S| == 2 && (exists n: Node :: n != removedNode && n in S) && S <= Union(edgesToChange) ;
+    assert |allIncidentNodes| > 0;
+    var maxNode: Node := pickMax(allIncidentNodes);
+    assert maxNode in allIncidentNodes;
+    var pickedEdge: Edge := {removedNode, maxNode};
+    assert exists edge: Edge :: edge in edgesToChange && maxNode in edge && removedNode in edge && |edge| == 2;
+    assert exists edge: Edge :: edge in edgesToChange && edge >= {removedNode, maxNode};
+    cardinalityLemma2();
+    assert exists edge: Edge :: edge in edgesToChange && edge == pickedEdge;
+    assert pickedEdge in edgesToChange;
+    pickedEdge
+}
+
+//Returns a set of nodes of cardinality equal to v's degree not contained in graph.0 
+function addedSplitNodes(graph: Graph, v: Node): (S: set<Node>)
+requires isValidGraph(graph) 
+{
+    if v in graph.0 && (exists e: Edge | e in graph.1 :: v in e ) then 
+        //The vertex is "split" such that all those edges still exist but connect to different new nodes
+        var neighbors: set<Node> := neighborsOf(graph, v);
+        var newNodes: set<Node> := addMultipleGreater(graph.0, |neighbors|); 
+        newNodes
+    //If the vertex does not belong to the graph or the vertex is not present in any edge, there are no new nodes
+    else {}
+}
+
+//The grapg resulting from removing a vertex is valid
+lemma removeVertexValid(g: Graph, v: Node)
+requires isValidGraph(g)
+requires v in g.0
+ensures isValidGraph((g.0 - {v}, g.1 - incidentEdges(g, v)))
+{
+    assert forall e | e in g.1 :: (|e| == 2 && exists u,v :: u in g.0 && v in g.0 && u != v && e == {u,v}); 
+}
+
+
+//A vertex that does not belong to graph.0 belongs to no edges in graph.1
+lemma notAVertexImpliesNotInAnEdge(graph: Graph, n: Node)
+requires isValidGraph(graph)
+requires n !in graph.0
+ensures forall e: Edge | e in graph.1 :: n !in e
+{ }
+
+//Same as above, but with a set of vertices
+lemma notAVertexImpliesNotInAnEdgeSet(graph: Graph, S: set<Node>)
+requires isValidGraph(graph)
+requires forall n: Node | n in S :: n !in graph.0
+ensures forall e: Edge, n: Node | e in graph.1 && n in S :: n !in e
+{ }
+
+*/
