Especificaciones/Envasado/EnvasadoProperties.dfy
@@ -1,0 +1,74 @@
+include "EnvasadoOpt.dfy"
+
+lemma boundoptimalValueEnvasado(A : multiset<nat>, E : nat, I:multiset<multiset<nat>>) 
+requires optimalEnvasado(A,E,I)
+ensures |I| <= |A|
+{ if (forall a | a in A :: a <= E)
+   {boundEnvasar(A,E);
+    assert envasarDecissionProblem(A,E,|A|);
+   }
+   else { 
+    noEnvasar(A,E);
+   }
+}
+
+lemma lowerBoundoptimalValueEnvasado(A : multiset<nat>, E : nat, I:multiset<multiset<nat>>) 
+requires optimalEnvasado(A,E,I)
+ensures |I| * E >= |A|
+{ 
+  var totalSumA: nat := SumNat(A);
+  assert forall m: multiset<nat> | m in I :: GSumNat(m) <= E;
+  
+  assume false; 
+}
+
+lemma isInEnvasado(A : multiset<nat>, a:nat, E : nat, I:multiset<multiset<nat>>)
+requires a in A && isEnvasado(A,E,I)
+ensures exists i :: i in I && a in i
+{
+  if (!exists i :: i in I && a in i)
+  { //assert Union(I) == A;
+    inOneUnion(I,a);
+    //assert !(a in A); //contradiction
+  }
+}
+
+lemma noEnvasar(A:multiset<nat>, E:nat)
+requires exists a :: a in A && a > E
+ensures ! exists I:multiset<multiset<nat>> :: isEnvasado(A,E,I)
+{if (exists I:multiset<multiset<nat>> :: isEnvasado(A,E,I))
+ {
+  var a:| a in A && a > E;
+  var I :| isEnvasado(A,E,I);
+  isInEnvasado(A,a,E,I);
+  var i :| i in I && a in i;
+  GSumNatElemIn(i,a);
+  assert GSumNat(i) >= a > E;
+ }
+
+}
+
+lemma boundEnvasar(A:multiset<nat>, E:nat)
+requires forall a | a in A :: a <= E
+ensures forall j | j >= |A| :: envasarDecissionProblem(A,E,j)
+{ 
+  var I:multiset<multiset<nat>> := multiset{};
+  var A':multiset<nat> := A;
+  while A' != multiset{}
+    invariant |I| == |A| - |A'|
+    invariant Union(I) == A-A'
+    invariant forall x | x in I :: x <= A && GSumNat(x) <= E
+   { var oldI := I;
+     var oldA' := A';
+
+    var a :| a in A';
+    I := I + multiset{multiset{a}};
+    A' := A' - multiset{a};
+    assert A - A' == A - oldA' + multiset{a};
+    UnionOne(I,multiset{a});
+    assert oldI == I - multiset{multiset{a}};
+    assert Union(I) == Union(oldI) + multiset{a};
+   }
+   assert |I| == |A|;
+   assert isEnvasado(A,E,I);
+}
