Turing Reducciones/VertexCover/PDVCToPOVC.dfy
@@ -1,7 +1,6 @@
 include "../../Especificaciones/VertexCover/VertexCoverOpt.dfy"
 
 
-
 //We assume a polynomial algorithm for POCV
 method {:axiom} moptimalVertexCover (graph : Graph) returns (I:set<Node>)
   requires isValidGraph(graph)
@@ -10,7 +9,7 @@ method {:axiom} moptimalVertexCover (graph : Graph) returns (I:set<Node>)
 //We implement a polynomial algorithm for PDCV using moptimalVertexCover
 method mVertexCover (graph:Graph, k:int) returns (b:bool)
   requires isValidGraph(graph)
-  ensures b == VertexCoverDecissionProblem(graph,k)
+  ensures b == vertexCoverDecissionProblem(graph,k)
 {
   var I := moptimalVertexCover(graph);
   //assert I <= graph.0 && isVertexCover(I,graph);
