Turing Reducciones/VertexCover/POCVToPCVRemoveVertex.dfy
@@ -1,49 +1,18 @@
 include "../../Especificaciones/VertexCover/VertexCoverOpt.dfy"
 include "../../Especificaciones/VertexCover/VertexCoverProperties.dfy"
-//include "../../Especificaciones/VertexCover/OptimalCoverPropertiesRemoveVertex.dfy"
 include "RemoveVertexAux.dfy"
 
-ghost predicate invariantLoop(
-  graph: Graph, okg: nat,
-  vertex: set<Node>,//remaining vertex
-  I: set<Node>, //up to now vertex cover
-  g: Graph, kg: nat//current graph
-)
-requires isValidGraph(graph)
-{
- isValidGraph(g) &&
- vertex <= g.0 &&
-//I is disjoint from vertex and from g
-//Vertex in g either have not been visited, so they belong to vertex
-//or have a non-covered edge  
- I <= graph.0 - vertex && I + g.0 == graph.0 &&
- I * g.0 == {} && I * vertex == {} &&
 
-//the union of all the edges covered by I and those in g.1 are 
-//the edges in the original graph
-//So at the end, when g.1 is empty, all the edges in graph are covered by I
-
- g.1 +  (set edge:Edge, node:Node | edge in graph.1 && node in I && node in edge :: edge) == graph.1 &&
- 
-//At the end kg = 0 and |I| = okg, so I is optimal
- kg >= 0 && optimalValueVertexCover(g,kg) &&
- kg + |I| == okg &&
-
- (forall u, O | u in g.0 && u !in vertex &&  I <= O <= graph.0 && isVertexCover(O,graph) && |O| == okg :: u !in O) &&
- (exists V : set<Node> :: V <= g.0 && V <= vertex && optimalVertexCover(g,V) && optimalVertexCover(graph, I + V))
-}
-
-//We assume a polynomial algorithm for PCV
+//We assume a polynomial algorithm for PVC
 method {:axiom} moptimalValueVertexCover (graph : Graph) returns (k: nat)
   requires isValidGraph(graph)
   ensures optimalValueVertexCover(graph,k)
 
-
 method bodyLoop(
-  ghost graph : Graph, ghost okg : nat,
-  vertex : set<Node>,//remaining vertex
-  I : set<Node>, //up to now vertex cover
-  g : Graph, kg : nat//current graph
+  ghost graph: Graph, ghost okg: nat,
+  vertex: set<Node>,//remaining vertex
+  I: set<Node>, //up to now vertex cover
+  g: Graph, kg : nat//current graph
 ) returns 
 (
   vertexn : set<Node>,//remaining vertex
@@ -98,6 +67,38 @@ ensures vertexn < vertex //in order to prove termination
       kgn := kg;  
     }
 }
+
+ghost predicate invariantLoop(
+  graph: Graph, okg: nat,
+  vertex: set<Node>,//remaining vertex
+  I: set<Node>, //up to now vertex cover
+  g: Graph, kg: nat//current graph
+)
+requires isValidGraph(graph)
+{
+ isValidGraph(g) &&
+ vertex <= g.0 &&
+//I is disjoint from vertex and from g
+//Vertex in g either have not been visited, so they belong to vertex
+//or have a non-covered edge  
+ I <= graph.0 - vertex && I + g.0 == graph.0 &&
+ I * g.0 == {} && I * vertex == {} &&
+
+//the union of all the edges covered by I and those in g.1 are 
+//the edges in the original graph
+//So at the end, when g.1 is empty, all the edges in graph are covered by I
+
+ g.1 +  (set edge:Edge, node:Node | edge in graph.1 && node in I && node in edge :: edge) == graph.1 &&
+ 
+//At the end kg = 0 and |I| = okg, so I is optimal
+ kg >= 0 && optimalValueVertexCover(g,kg) &&
+ kg + |I| == okg &&
+
+ (forall u, O | u in g.0 && u !in vertex &&  I <= O <= graph.0 && isVertexCover(O,graph) && |O| == okg :: u !in O) &&
+ (exists V : set<Node> :: V <= g.0 && V <= vertex && optimalVertexCover(g,V) && optimalVertexCover(graph, I + V))
+}
+
+
 
 
 
